# Series expansion

```{example} Taylor series
Find the two-term Taylor series for

\begin{equation}
f(x) = xe^{2 x^2}
\end{equation}

about $x = 0$.

---

We will evaluate the required derivatives. This will be a series of
[product rule](derivative-rules.md) calculations.

The value of the function is $f(0) = 0$. The first derivative is:

\begin{align}
f'(x) &= x(e^{2x^2}4x) + e^{2x^2} \\
&= (4x^2 + 1)e^{2x^2}
\end{align}
so $f'(0) = 1$. The second derivative is:

\begin{align}
f''(x) &= (4x^2+1)(e^{2x^2}4x)+8xe^{2x^2} \\
&= (16x^3+12x)e^{2x^2}
\end{align}
so $f''(0) = 0$. This means we need to keep going! The third derivative is:

\begin{align}
f'''(x) &= (16x^3+12x)(e^{2x^2}4x)+(48x^2+12)e^{2x^2} \\
&= (64x^4+96x^2+12)e^{2x^2}
\end{align}
so $f'''(0) = 12$.

Putting it all together,

\begin{equation}
f(x) \approx 0 + 1 \cdot x + \frac{1}{2} \cdot 0 \cdot x^2
+ \frac{1}{6} \cdot 12 \cdot x^3 + \cdots = x + 2x^3 + \cdots
\end{equation}

````

## Combining series

Some of these calculations can sometimes be avoided by combining series
together. For example, the Taylor series for $e^x$ is well known

\begin{equation}
e^x = \sum_{n=0}^{\infty} \frac{x^n}{n!} = 1 + x + \frac{x^2}{2} + \cdots
\end{equation}

The argument of *e* in *f* is $2x^2$, which is also zero when *x* is zero, so we
can substitute it in the known series to obtain

\begin{equation}
e^{2x^2} \approx 1 + 2x^2 + \frac{(2x^2)^2}{2} + \cdots
\end{equation}

Finally, inserting this series into *f* and expanding

\begin{align}
f(x) &= x e^{2x^2} \approx x (1 + 2x^2 + 2x^4 + \cdots) \\
&= x + 2x^3 + \cdots
\end{align}

When doing this process, it can be helpful to keep track of dropped terms using
$O$-notation

\begin{align}
e^x &= \sum_{n=0}^{\infty} \frac{x^n}{n!} = 1 + x +  \frac{x^2}{2} + O(x^3) \\
e^{2x^2} &= 1 + 2x^2 + 2x^4 + O(x^6) \\
xe^{2x^2} &= x + 2x^3 + O(x^5)
\end{align}

## Skill builder problems

Expand the following to two terms:

(a) $f(x)=\cos(x)$ at $x=0$

The derivatives are:

\begin{align}
f'(x)&=-\sin(x)\\
f''(x)&=-\cos(x)
\end{align}

Evaluating everything at $x=0$:

\begin{align}
f(0)=1\\
f'(0)=0\\
f''(0)=-1
\end{align}

So:

\begin{equation}
f(x) \approx 1-\frac{x^2}{2}
\end{equation}

(b) $f(x)=\sin(x)$ at $x=0$

The derivatives are:

\begin{align}
f(x)&=\sin(x)\\
f'(x)&=\cos(x)\\
f''(x)&=-\sin(x)\\
f^{(3)}(x)&=-\cos(x)
\end{align}

Evaluating at $x=0$:
\begin{align}
f(0)=0\\
f'(0)=1\\
f''(0)=0\\
f^{3}(0)=-1
\end{align}

So:

\begin{equation}
f(x) \approx x-\frac{x^3}{6}
\end{equation}

(c) $f(x)=e^x$ at $x=0$

Derive and evaluate:

\begin{align}
f(x)&=e^x \rightarrow f(0)=1\\
f'(x)&=e^x \rightarrow f'(0)=1
\end{align}

So:

\begin{equation}
f(x) \approx 1+x
\end{equation}

(d) $f(x)=\ln(1+x)$ at $x=0$

Derive and Evaluate:

\begin{align}
f(x)&=\ln(1+x) \rightarrow f(0)=0\\
f'(x)&=\frac{1}{1+x} \rightarrow f'(0)=1\\
f''(x)&=-\frac{1}{(1+x)^2} \rightarrow f''(0)=-1
\end{align}

So:

\begin{equation}
f(x) \approx x-\frac{x^2}{2}
\end{equation}

(e) $f(x)=\frac{1}{1+x}$ at $x=0$

Derive and Evaluate:

\begin{align}
f(x)&=\frac{1}{1+x} \rightarrow f(0)=1\\
f'(x)&=-\frac{1}{(1+x)^2} \rightarrow f'(0)=1
\end{align}

So:

\begin{equation}
f(x) \approx 1-x
\end{equation}

(f) $f(x)=\cos(4x)$ at $x=0$

From part (a) we found...

\begin{equation}
f(x)=cos(x) \approx 1-\frac{x^2}{2}
\end{equation}

We can find the Taylor series of a function $f(ax)$ by substituting $ax$ for $x$
in the Taylor series for $f(x)$.

So:

\begin{equation}
f(x)=\cos(4x) \approx 1-\frac{(4x)^2}{2} \approx 1-8x^2
\end{equation}

(g) $f(x)=\cos(x-\pi)$ at $x=\pi$

We can use the same method used to solve part (f).

\begin{equation}
f(x)=cos(x) \approx 1-\frac{x^2}{2}
\end{equation}

So:

\begin{equation}
f(x)=\cos(x-\pi) \approx 1-\frac{(x-\pi)^2}{2}
\end{equation}

Note: There is a constant shift of $x$ and $x_0$

(h) $f(x)=e^x \sin(x)$ at $x=0$

To find the Taylor expansion of the product of two functions, f(x)Â·g(x), you may
multiply their individual Taylor series expansions.

Recall:

The Taylor expansion of $f(x)=e^x$ is $f(x) \approx 1+x$

The Taylor expansion of $f(x)=\sin(x)$ is $f(x) \approx x-\frac{x^3}{6}$

So:

\begin{equation}
f(x) \approx (1+x+\dots)(x-\frac{x^3}{6}+\dots) \approx x+x^2
\end{equation}

(i) $f(x)=\cos(x)$ at $x=\pi$

Note: Reuse derivatives from part (a) but evaluate at $\pi$ instead of zero.

\begin{align}
f(\pi)=-1\\
f'(\pi)=0\\
f''(\pi)=1
\end{align}

\begin{equation}
f(x) \approx -1+\frac{1}{2}(x-\pi)^2
\end{equation}

(j) $f(x)=7x^2-6x+1$ at $x=2$

\begin{align}
f(x)&=7x^2-6x+1 \rightarrow f(2)=17\\
f'(x)&=14x-6 \rightarrow f'(2)=22
\end{align}

\begin{equation}
f(x) \approx 17+22(x-2)
\end{equation}
